firmware/IncrementWait/IncrementWaitToCava.v
@@ -3,6 +3,7 @@ Require Import Coq.ZArith.ZArith. Open Scope Z_scope.
 Require Import Coq.Strings.String. Open Scope string_scope.
 Require Import coqutil.Byte.
 Require Import coqutil.Word.Interface coqutil.Word.Properties.
+Require Import coqutil.Tactics.fwd.
 Require Import bedrock2.ZnWords.
 Require Import compiler.SeparationLogic.
 Require Import Bedrock2Experiments.RiscvMachineWithCavaDevice.ExtraRiscvMachine.
@@ -14,56 +15,65 @@ Require Import Bedrock2Experiments.RiscvMachineWithCavaDevice.Bedrock2ToCava.
 
 Definition binary: list byte := Eval compute in Pipeline.instrencode put_wait_get_asm.
 
-Theorem IncrementWait_end2end_correct: forall p_functions p_call mH Rdata Rexec R (* <-? *)
-          (initialL: ExtraRiscvMachine counter_device) input output_placeholder sched,
-    -2^19 <= word.signed (word.sub p_functions p_call) < 2^19 ->
-    128 <= word.unsigned (word.sub stack_pastend stack_start) ->
+Theorem IncrementWait_end2end_correct: forall p_functions ret_addr mH (Rdata Rexec R: mem -> Prop)
+          (initialL: ExtraRiscvMachine counter_device) input sched,
     word.unsigned (word.sub stack_pastend stack_start) mod 4 = 0 ->
     word.unsigned p_functions mod 4 = 0 ->
-    word.unsigned p_call mod 4 = 0 ->
+    word.unsigned ret_addr mod 4 = 0 ->
+    machine_ok p_functions stack_start stack_pastend binary mH Rdata Rexec initialL ->
+    R mH ->
+    map.get initialL.(getRegs) RegisterNames.a0 = Some input ->
+    map.get initialL.(getRegs) RegisterNames.ra = Some ret_addr ->
+    word.unsigned ret_addr mod 4 = 0 ->
     initialL.(getLog) = [] ->
-    machine_ok p_functions main_relative_pos stack_start stack_pastend binary p_call
-               p_call mH Rdata Rexec initialL ->
-    (scalar (word.of_Z input_ptr) input * scalar (word.of_Z output_ptr) output_placeholder * R)%sep mH ->
+    initialL.(getPc) = word.add p_functions (word.of_Z put_wait_get_relative_pos) ->
     exists steps_remaining finalL mH',
       run sched steps_remaining initialL = (Some tt, finalL) /\
-      machine_ok p_functions main_relative_pos stack_start stack_pastend binary p_call
-                 (word.add p_call (word.of_Z 4)) mH' Rdata Rexec finalL /\
-      (scalar (word.of_Z input_ptr) input *
-       scalar (word.of_Z output_ptr) (word.add (word.of_Z 1) input) * R)%sep mH' /\
+      machine_ok p_functions stack_start stack_pastend binary mH' Rdata Rexec finalL /\
+      R mH' /\
+      map.get finalL.(getRegs) RegisterNames.a0 = Some (word.add (word.of_Z 1) input) /\
+      finalL.(getPc) = ret_addr /\
       finalL.(getLog) = initialL.(getLog) (* no external interactions happened *).
 Proof.
   intros.
   change binary with (Pipeline.instrencode put_wait_get_asm).
-  refine (bedrock2_and_cava_system_correct
-            _ _ _ _ _ _ _ _ _ _ _ _ _ _ _ _ _ _ _ _ _ _ _ _ _ _ _ _ _ _ _ _ _);
-    try eassumption.
+  edestruct bedrock2_and_cava_system_correct with
+      (f_entry_name := "put_wait_get")
+      (stack_start := stack_start) (stack_pastend := stack_pastend)
+      (postH := fun m' retvals =>  R m' /\ retvals = [word.add (word.of_Z 1) input])
+    as (steps_remaining & finalL & mH' & retvals & Rn & GM & A & Eq & M & HP & HL);
+    lazymatch goal with
+    | |- _ mod _ = _ => idtac
+    | |- _ => try eassumption
+    end.
   { exact funcs_valid. }
-  { apply List.dedup_NoDup_iff with (aeqb_spec:=String.eqb_spec). reflexivity. }
+  { apply List.dedup_NoDup_iff. reflexivity. }
   { exact put_wait_get_compile_result_eq. }
   { (* check that the compiler emitted valid instructions: *)
     repeat (apply Forall_cons || apply Forall_nil).
     all: vm_compute; try intuition discriminate. }
-  { unfold main_relative_pos.
-    match goal with
-    | H: _ <= ?x < _ |- _ <= _ + ?x' < _ => change x' with x
-    end.
-    Lia.lia. }
-  { instantiate (2 := "main"). reflexivity. }
   { reflexivity. }
-  { ZnWords. }
-  { refine (WeakestPreconditionProperties.Proper_cmd _ _ _ _ _ _ _ _ _ _ _).
-    1: eapply WeakestPreconditionProperties.Proper_call.
-    2: {
-      eapply main_correct. 1: eassumption.
-      match goal with
-      | H: ?t = ?t' |- _ ?t'' _ => replace t'' with t' by exact H
-      end.
-      reflexivity. }
-    unfold post_main.
-    repeat intro. Tactics.logical_simplify. Tactics.ssplit. 1: eassumption.
-    eexists. split; [eassumption|reflexivity].
-  }
+  { vm_compute. discriminate. }
+  { assumption. }
+  { assumption. }
+  { assumption. }
+  { eapply WeakestPreconditionProperties.Proper_call.
+    2: eapply IncrementWaitProperties.put_wait_get_correct.
+    2: eassumption.
+    2: reflexivity.
+    unfold Morphisms.pointwise_relation, Basics.impl.
+    intros. fwd.
+    unfold IncrementWaitSemantics.proc.
+    split. 1: split; [assumption|reflexivity].
+    eexists; split; [eassumption|reflexivity]. }
+  { cbn -[map.get].
+    match goal with
+    | H: map.get _ RegisterNames.a0 = Some input |-
+      match ?x with _ => _ end = _ => replace x with (Some input)
+    end.
+    reflexivity. }
+  { eassumption. }
+  { cbn -[map.get] in GM. fwd. eauto 10. }
 Qed.
 
 (* Goal: bring this list down to only standard axioms like functional and propositional extensionality
